src/ConstraintTreeTypes.v
@@ -1,0 +1,25 @@
+Require Import Arith.
+Require Import List.
+Require Import String.
+Require Import Ascii.
+Require Import PipeGraph.Debug.
+Require Import PipeGraph.Util.
+Require Import PipeGraph.StringUtil.
+Require Import PipeGraph.Instruction.
+Require Import PipeGraph.Graph.
+Require Import PipeGraph.FOLPredicate.
+Require Import PipeGraph.GraphvizCompressed.
+
+Inductive ScenarioTree : Set :=
+| ScenarioName : string -> ScenarioTree -> ScenarioTree
+| ScenarioAxiomName : string -> ScenarioTree -> ScenarioTree
+| ScenarioAnd : ScenarioTree -> ScenarioTree -> ScenarioTree
+| ScenarioOr : ScenarioTree -> ScenarioTree -> ScenarioTree
+| ScenarioEdgeLeaf : list GraphEdge -> ScenarioTree
+| ScenarioNotEdgeLeaf : list GraphEdge -> ScenarioTree
+| ScenarioNodeLeaf : list GraphNode -> ScenarioTree
+| ScenarioNotNodeLeaf : list GraphNode -> ScenarioTree
+| ScenarioLoadConstraint : Microop -> Data -> bool -> ScenarioTree
+| ScenarioTrue : ScenarioTree
+| ScenarioFalse : ScenarioTree.
+
