src/VscaleMappings.v
@@ -1,0 +1,470 @@
+Require Import Arith.
+Require Import List.
+Require Import String.
+Require Import Ascii.
+Require Import PipeGraph.Debug.
+Require Import PipeGraph.Util.
+Require Import PipeGraph.StringUtil.
+Require Import PipeGraph.Instruction.
+Require Import PipeGraph.Graph.
+Require Import PipeGraph.FOLPredicate.
+Require Import PipeGraph.GraphvizCompressed.
+Require Import PipeGraph.ConstraintTreeTypes.
+
+Open Scope string_scope.
+
+Import ListNotations.
+
+Definition ToString
+  (n : nat)
+  : string :=
+  stringOfNat n.
+
+Definition GetBaseIndex
+  (c : nat)
+  : nat :=
+  match c with
+  | 0 => 1
+  | 1 => 6
+  | 2 => 11
+  | 3 => 16
+  | _ => Warning 1 ["Trying to get base mem index of an undefined core!"]
+  end.
+
+
+Definition GetPCofMicroop
+  (uop : Microop)
+  (bases : list (nat * nat))
+  : string :=
+  let c := coreID uop in
+  let t := match (find (fun x => beq_nat c (fst x)) bases) with
+           | None => Warning 0 ["Could not find base PC for core "; ToString c]
+           | Some (c', b) => (globalID uop) - b
+           end
+  in
+  ToString (((GetBaseIndex c) * 4) + (t * 4)).
+
+
+(* We don't technically need to pass along the core for these functions, but it makes things easier. *)
+Definition MapFetch
+  (uop : Microop)
+  (core : nat)
+  (bases : list (nat * nat))
+  : list string :=
+  ["core_gen_block["; ToString core; "].vscale.pipeline.PC_IF == 32'd"; GetPCofMicroop uop bases;
+    " && ~(core_gen_block["; ToString core; "].vscale.pipeline.stall_IF || core_gen_block["; ToString core; "].vscale.pipeline.kill_IF)"].
+
+Definition MapDecEx
+  (uop : Microop)
+  (core : nat)
+  (bases : list (nat * nat))
+  : list string :=
+  ["core_gen_block["; ToString core; "].vscale.pipeline.PC_DX == 32'd"; GetPCofMicroop uop bases; " && ~(core_gen_block["; ToString core; "].vscale.pipeline.stall_DX)"].
+
+Definition MapWB
+  (uop : Microop)
+  (core : nat)
+  (bases : list (nat * nat))
+  (lc: list ScenarioTree)
+  : list string :=
+  let base_prop :=
+      ["core_gen_block["; ToString core; "].vscale.pipeline.PC_WB == 32'd"; GetPCofMicroop uop bases; " && ~(core_gen_block[";
+      ToString core; "].vscale.pipeline.stall_WB)"] in
+  let f x := match x with
+             | ScenarioLoadConstraint op _ _ => beq_uop op uop
+             | _ => false
+             end in
+  match find f lc with
+  | Some x => match x with
+              | ScenarioLoadConstraint op dat neg =>
+                    let eq_str := if neg then "!=" else "==" in
+                    match dat with
+                    | NormalData n =>
+                        app base_prop [" && core_gen_block["; ToString core; "].vscale.pipeline.load_data_WB "; eq_str; " 32'd"; ToString n]
+                    | _ => Warning base_prop ["Something other than NormalData here!"]
+                    end
+              | _ => Warning base_prop ["Should have gotten a ScenarioLoadConstraint but got something else!"]
+              end
+  | None => base_prop
+  end.
+
+(* Node mapping function for Vscale. *)
+Definition MapNodeVscale
+  (n : GraphNode)
+  (bases : list (nat * nat))
+  (lc: list ScenarioTree)
+  : list string :=
+  let (uop, loc) := n in
+  let (_, stage) := loc in
+  let core := coreID uop in
+  match stage with
+  (* Fetch *)
+  | 0 => MapFetch uop core bases
+  (* DecodeExecute *)
+  | 1 => MapDecEx uop core bases
+  (* Writeback *)
+  | 2 => MapWB uop core bases lc
+  | _ => Warning [] ["Trying to map undefined stage!"]
+  end.
+
+Definition GetMemIndexForAddr
+  (for_reg : bool)
+  (n : nat)
+  : nat :=
+  if for_reg then (84 + (n * 4)) else (21 + n).
+
+Fixpoint GetAddresses
+  (l : list Microop)
+  (addrs : list PhysicalAddress)
+  : list PhysicalAddress :=
+  let get_addr x :=
+        match x with
+        | Read _ _ a _ => Some a
+        | Write _ _ a _ => Some a
+        | _ => None
+        end
+  in
+  match l with
+  | [] => addrs
+  | h::t => match (get_addr (access h)) with
+            | None => GetAddresses t addrs
+            | Some a => if (find (beq_paddr a) addrs) then GetAddresses t addrs else GetAddresses t (a::addrs)
+            end
+  end.
+
+Fixpoint GetInitialConditionMapping
+  (conditions : list BoundaryCondition)
+  (pa : PhysicalAddress)
+  : Data :=
+  match conditions with
+  | (a, d) :: t =>
+      if beq_paddr a pa
+      then d
+      else GetInitialConditionMapping t pa
+  | [] =>
+      let result := NormalData 0 in
+      if PrintFlag 6
+      then Comment result
+        ["Using implicit initial condition data=0 for PA: ";
+        GraphvizStringOfPhysicalAddress pa]
+      else result
+  end.
+
+Definition FindInitialState
+  (init: list BoundaryCondition)
+  (addr : PhysicalAddress)
+  : (PhysicalAddress * Data) :=
+  (addr, (GetInitialConditionMapping init addr)).
+
+Fixpoint AddToThread
+  (uop : Microop)
+  (l : list (nat * (list Microop)))
+  : list (nat * (list Microop)) :=
+  match l with
+  | [] => [((coreID uop), [uop])]
+  | h::t => if (beq_nat (coreID uop) (fst h)) then ((fst h), (app (snd h) [uop]))::t else h::(AddToThread uop t)
+  end.
+
+Fixpoint FilterUops
+  (l : list Microop)
+  (l' : list (nat * (list Microop)))
+  : list (nat * (list Microop)) :=
+  match l with
+  | [] => l'
+  | h::t => FilterUops t (AddToThread h l')
+  end.
+
+(* For halt logic. *)
+Fixpoint AddCoreUopList
+  (n : nat)
+  (l : list (nat * (list Microop)))
+  : list (nat * (list Microop)) :=
+  match l with
+  | [] => [(n, [])]
+  | h::t => if beq_nat (fst h) n then l else h::(AddCoreUopList n t)
+  end.
+
+Fixpoint EnsureCores
+  (max_core_id : nat)
+  (l : list (nat * (list Microop)))
+  : list (nat * (list Microop)) :=
+  match max_core_id with
+  | 0 => AddCoreUopList max_core_id l
+  | S n' => EnsureCores n' (AddCoreUopList max_core_id l)
+  end.
+
+Fixpoint FindAddressReg
+  (base : nat)
+  (addrs : list (nat * nat))
+  (tag : nat)
+  : (nat * (nat * (list (nat * nat)))) :=
+  match addrs with
+  | [] => (base, ((S base), ((tag, base)::addrs)))
+  | h::t => if beq_nat tag (fst h) then ((snd h), (base, addrs)) else FindAddressReg base t tag
+  end.
+
+Fixpoint GetMemIndexOf
+  (uop : Microop)
+  (bases : list (nat * nat))
+  : nat :=
+  let c := coreID uop in
+  let t := match (find (fun x => beq_nat c (fst x)) bases) with
+           | None => Warning 0 ["Could not find base mem index for core "; ToString c]
+           | Some (c', b) => (globalID uop) - b
+           end
+  in
+  (GetBaseIndex c) + t.
+
+Fixpoint MapInitMemInstrsHelper
+  (assume_outer : string)
+  (bases : list (nat * nat))
+  (thread : list Microop)
+  (base : nat) (* the reg to use next *)
+  (l : list (nat * nat)) (* which registers have been used for which address *)
+  (assums : list string)
+  (regs : list (nat * nat)) (* reg * value *)
+  (cur_index : nat) (* the index to use for the halt instruction *)
+  : (list (nat * nat) * (list string)) := (* core * reg * value *)
+  let f d :=
+      match d with
+      | NormalData n => n
+      | _ => Warning 0 ["Found something other than NormalData!"]
+      end
+  in
+  let g d :=
+      match d with
+      | PTag n => n
+      | _ => Warning 0 ["Found something other than PTag!"]
+      end
+  in
+  match thread with
+  | [] => let assums := app assums [assume_outer; "hasti_mem.mem["; ToString cur_index;
+                                    "] == `RV32_HALT);"; newline] in
+        (regs, assums)
+  | h::t =>
+        match access h with
+        | Write _ _ a d =>
+              let (tag, index) := a in
+              let tag := g tag in
+              let (cur, bl) := FindAddressReg base l tag in (* For the address reg *)
+              let (base', l') := bl in
+              MapInitMemInstrsHelper assume_outer bases t (S base') l' (app assums [assume_outer; "hasti_mem.mem["; ToString (GetMemIndexOf h bases);
+               "] == {7'b0,5'd"; ToString base'; ",5'd"; ToString cur; ",3'd2,5'b0,`RV32_STORE});"; newline])
+               (app ((cur, GetMemIndexForAddr true tag)::regs) [(base', f d)]) (* This trickery is deliberate. I want the data assumptions to be at the end. *)
+               (S (GetMemIndexOf h bases))
+        | Read _ _ a d =>
+              let (tag, index) := a in
+              let tag := g tag in
+              let (cur, bl) := FindAddressReg base l tag in (* For the address reg *)
+              let (base', l') := bl in
+              MapInitMemInstrsHelper assume_outer bases t (S base') l' (app assums [assume_outer; "hasti_mem.mem["; ToString (GetMemIndexOf h bases);
+               "] == {12'b0,5'd"; ToString cur; ",3'd2,5'd"; ToString base'; ",`RV32_LOAD});"; newline]) ((cur, GetMemIndexForAddr true tag)::regs) (S (GetMemIndexOf h bases))
+        | Fence _ =>
+              MapInitMemInstrsHelper assume_outer bases t base l (app assums [assume_outer; "hasti_mem.mem["; ToString (GetMemIndexOf h bases);
+               "] == {4'b0,8'b1,5'b0,3'b`RV32_FUNCT3_FENCE,5'b0,`RV32_MISC_MEM});"; newline]) regs (S (GetMemIndexOf h bases))
+        | _ => Warning ([], []) ["Mapping an instr other than a load/store/fence!"]
+        end
+  end.
+
+Fixpoint AddCoreID
+  (n : nat)
+  (l : list (nat * nat))
+  : list (nat * (nat * nat)) :=
+  match l with
+  | [] => []
+  | h::t => (n, h)::(AddCoreID n t)
+  end.
+
+Definition MapInitMemInstrs
+  (assume_outer : string)
+  (bases : list (nat * nat))
+  (threads : nat * (list Microop))
+  : (list (nat * (nat * nat)) * (list string)) := (* core * reg * value *)
+  let t := (MapInitMemInstrsHelper assume_outer bases (snd threads) 1 [] [] [] (GetBaseIndex (fst threads))) in
+  ((AddCoreID (fst threads) (fst t)), (snd t)).
+
+Definition GetAssumptionsFromTuples
+  (l1 : list string)
+  (l2 : list (nat * (nat * nat)) * (list string))
+  : list string :=
+  app l1 (snd l2).
+
+Definition GetRegsFromTuples
+  (l1 : list (nat * (nat * nat)))
+  (l2 : list (nat * (nat * nat)) * (list string))
+  : list (nat * (nat * nat)) :=
+  app l1 (fst l2).
+
+Definition TranslateAddrInits
+  (assume_outer : string)
+  (tup: PhysicalAddress * Data)
+  : list string :=
+  let f d :=
+      match d with
+      | NormalData n => n
+      | _ => Warning 0 ["Found something other than NormalData!"]
+      end
+  in
+  let g d :=
+      match d with
+      | PTag n => n
+      | _ => Warning 0 ["Found something other than PTag!"]
+      end
+  in
+  [assume_outer; "hasti_mem.mem["; ToString (GetMemIndexForAddr false (g (ptag (fst tup)))); "] == {32'd"; ToString (f (snd tup)); "});"; newline].
+
+Definition TranslateInitReg
+  (assume_outer : string)
+  (tup : nat * (nat * nat)) (* core * reg * data *)
+  : list string :=
+  [assume_outer; "core_gen_block["; ToString (fst tup);
+  "].vscale.pipeline.regfile.data["; ToString (fst (snd tup)); "] == 32'd"; ToString (snd (snd tup)); ");"; newline].
+
+Definition MapAssumptions
+  (assume_outer : string)
+  (bases : list (nat * nat))
+  (inits : list (PhysicalAddress * Data))
+  (threads : list (nat * (list Microop)))
+  : list string :=
+  let im := Map (MapInitMemInstrs assume_outer bases) threads in
+  let instr_mem_assums := fold_left GetAssumptionsFromTuples im [] in
+  let data_mem_assums := fold_left (fun x y => app x y) (Map (TranslateAddrInits assume_outer) (rev inits)) [] in
+  let used_regs := fold_left GetRegsFromTuples im [] in
+  let regs_assums := fold_left (fun x y => app x y) (Map (TranslateInitReg assume_outer) used_regs) [] in
+  app (app instr_mem_assums data_mem_assums) regs_assums.
+
+Definition AddShadowState
+  (l : list string)
+  : list string :=
+  let l' := ["reg run_once_clk;"; newline; newline;
+             "always @(posedge clk) begin"; newline;
+             tab; "if (reset) begin"; newline;
+                tab; tab; "run_once_clk <= 0;"; newline;
+                   tab; "end else if (run_once_clk == 0) begin"; newline;
+                       tab; tab; "run_once_clk <= 1;"; newline;
+                         tab; "end"; newline;
+                            "end"; newline; newline] in
+
+  app l' l.
+
+Fixpoint PrintLoadValueAssumptionsHelper
+  (assume_outer : string)
+  (bases : list (nat * nat))
+  (l : list Microop)
+  (l' : list string)
+  : list string :=
+  let f x := match x with
+             | [] => true
+             | _ => false
+             end in
+  match l with
+  | [] => app (assume_outer::l') ["));"; newline]
+  | h::t => let str_add := if f t then ["))"] else [")) and "; newline] in 
+            match access h with
+            | Read _ _ a d =>
+                PrintLoadValueAssumptionsHelper assume_outer bases t (app l' (app (app ("(("::(MapWB h (coreID h) bases [])) (") |-> ("::(MapWB h (coreID h) bases [ScenarioLoadConstraint h d false]))) str_add))
+            | _ => PrintLoadValueAssumptionsHelper assume_outer bases t l'
+            end
+  end.
+
+Definition PrintLoadValueAssumptions
+  (assume_outer : string)
+  (bases : list (nat * nat))
+  (l : list Microop)
+  (l' : list string)
+  : list string :=
+  match l with
+  | [] => []
+  | _ => PrintLoadValueAssumptionsHelper assume_outer bases l l'
+  end.
+
+Definition GenFinalStatePrecond
+  (core : nat)
+  : list string :=
+  ["(core_gen_block["; ToString core; "].vscale.pipeline.halted == 1'b1 && core_gen_block["; ToString core; "].vscale.pipeline.PC_WB == 32'd120 && ~(core_gen_block[";
+  ToString core; "].vscale.pipeline.stall_WB))"].
+
+Definition AddAnd
+  (l : list string)
+  (l' : list string)
+  : list string :=
+  match l with
+  | [] => l'
+  | _ => app l (" && "::l')
+  end.
+
+Definition MapFinalStatePrecond
+  (rtl_map_fn : string)
+  (cores : list nat)
+  : list string :=
+  let str_cmp := beq_string rtl_map_fn "Vscale_TSO" in
+  match str_cmp with
+  | true => app ("("::(fold_left AddAnd (Map GenFinalStatePrecond cores) [])) [")"]
+  | _ => app ("("::(fold_left AddAnd (Map GenFinalStatePrecond cores) [])) [")"]
+  end.
+
+Definition MapFinalStateHelper
+  (b : BoundaryCondition)
+  : list string :=
+  let f d :=
+      match d with
+      | NormalData n => n
+      | _ => Warning 0 ["Found something other than NormalData!"]
+      end
+  in
+  let g d :=
+      match d with
+      | PTag n => n
+      | _ => Warning 0 ["Found something other than PTag!"]
+      end
+  in
+  ["hasti_mem.mem["; ToString (GetMemIndexForAddr false (g (ptag (fst b)))); "] == {32'd"; ToString (f (snd b)); "}"].
+
+Fixpoint MapFinalState
+  (l : list BoundaryCondition)
+  (l' : list string)
+  : list string :=
+  match l with
+  | [] => l'
+  | h::t => match l' with
+            | [] => MapFinalState t (app ("("::(MapFinalStateHelper h)) [")"])
+            | _  => MapFinalState t (app l' (" && "::(app ("("::(MapFinalStateHelper h)) [")"])))
+            end
+  end.
+
+
+Definition PrintFinalValueAssumptions
+  (rtl_map_fn : string)
+  (assume_outer : string)
+  (l : list BoundaryCondition)
+  (l' : list string)
+  : list string :=
+  (* We need to have the assumption be true in the case where there are NO final state conditions, hence the "1" in the call to MapFinalState. *)
+  let str_cmp := beq_string rtl_map_fn "Vscale_TSO" in
+  match str_cmp with
+  | true => app (app (assume_outer::(MapFinalStatePrecond rtl_map_fn [0; 1; 2; 3])) (" |-> ("::(MapFinalState l ["1"]))) [")));"]
+  | _ => app (app (assume_outer::(MapFinalStatePrecond rtl_map_fn [0; 1; 2; 3])) (" |-> ("::(MapFinalState l ["1"]))) [")));"]
+  end.
+
+(* The program mapping function for Vscale. *)
+Definition PrintRTLAssumptionsVscale
+  (bases : list (nat * nat))
+  (l : list Microop)
+  (unch_loads : list Microop)
+  (initial : list BoundaryCondition)
+  (final : list BoundaryCondition)
+  (rtl_map_fn : string)
+  : list string :=
+  let addrs := GetAddresses l [] in
+  let addr_inits := Map (FindInitialState initial) addrs in
+  let threads := FilterUops l [] in
+  let pad_threads := EnsureCores 3 threads in (* cores are zero-indexed... *)
+  let assume_outer := "assume property (@(posedge clk) ~run_once_clk |-> " in
+  let assume_outer' := "assume property (@(posedge clk) (" in
+  let f x := match access x with
+             | Read _ _ _ _ => true
+             | _ => false
+             end in
+  app (app (app (AddShadowState (MapAssumptions assume_outer bases addr_inits pad_threads)) (PrintLoadValueAssumptions assume_outer' bases (filter f unch_loads) []))
+    (PrintFinalValueAssumptions rtl_map_fn assume_outer' final [])) [newline].
+
