scripts/rtlcheck/FPV_template_full_proof.tcl
@@ -1,0 +1,79 @@
+# ----------------------------------------
+#  Copyright (C) 2014 Jasper Design Automation, Inc. All Rights
+#  Reserved.  Unpublished -- rights reserved under the copyright
+#  laws of the United States.
+# ----------------------------------------
+
+# Analyze design under verification files
+set ROOT_PATH <Vscale root directory>
+set RTL_PATH ${ROOT_PATH}/src/main/verilog/
+set PROP_PATH ${ROOT_PATH}/src/main/verilog/
+
+# Analyze property files
+analyze -sv09 \
+  ${PROP_PATH}/vscale_alu.v \
+  ${PROP_PATH}/vscale_ctrl.v \
+  ${PROP_PATH}/vscale_mul_div.v \
+  ${PROP_PATH}/vscale_regfile.v \
+  ${PROP_PATH}/vscale_core.v \
+  ${PROP_PATH}/vscale_hasti_bridge.v \
+  ${PROP_PATH}/vscale_PC_mux.v \
+  ${PROP_PATH}/vscale_src_a_mux.v \
+  ${PROP_PATH}/vscale_csr_file.v \
+  ${PROP_PATH}/vscale_imm_gen.v \
+  ${PROP_PATH}/vscale_pipeline.v \
+  ${PROP_PATH}/vscale_src_b_mux.v \
+  ${PROP_PATH}/vscale_arbiter.v \
+  ${PROP_PATH}/vscale_dp_hasti_sram.v \
+  ${PROP_PATH}/SIM_TOP_NAME
+
+# 15 minutes for compiling properties
+set_task_compile_time_limit 900
+set_property_compile_time_limit 900
+# Elaborate design and properties
+echo "Elaboration_start: " [date +%s]
+elaborate -top vscale_sim_top
+echo "Elaboration_end: " [date +%s]
+
+# Set up Clocks and Resets
+echo "Reset_start: " [date +%s]
+clock clk
+reset reset
+echo "Reset_end: " [date +%s]
+
+# Get design information to check general complexity
+echo "Design_info_start: " [date +%s]
+get_design_info
+echo "Design_info_end: " [date +%s]
+
+# Check assumptions, see if we get lucky
+# 1 hour max
+set_prove_time_limit 1h
+echo "Pass0_Start: " [date +%s]
+set_max_trace_length 50
+set_prove_per_property_time_limit 30s
+set_prove_per_property_time_limit_factor 2
+set_engine_mode {K I N C}
+prove -all -covers
+echo "Pass0_End: " [date +%s]
+echo "ASSUMPTION_PASS_REPORT_BEGIN"
+report
+echo "ASSUMPTION_PASS_REPORT_END"
+
+#
+# 2nd pass: Validation of remaining properties with different engine
+# 10 hours
+set_prove_time_limit 10h
+echo "Pass2_Start: " [date +%s]
+set_max_trace_length 50
+set_prove_per_property_time_limit 500s
+set_prove_per_property_time_limit_factor 2
+set_engine_mode {I N AD AM}
+prove -all -asserts
+echo "Pass2_End: " [date +%s]
+
+# Report proof results
+echo "PASS2_REPORT_BEGIN"
+report
+echo "PASS2_REPORT_END"
+exit
