scripts/rtlcheck/gen_props.sh
@@ -1,0 +1,26 @@
+#!/bin/bash
+
+rm -rf pc_out/*
+rm -rf sva/*
+rm -rf jobs/*
+rm -rf fpv/*
+rm -rf jg_out/*
+
+mkdir -p pc_out/
+mkdir -p sva/
+mkdir -p jobs/
+mkdir -p fpv/
+mkdir -p jg_out/
+
+for file in $(find "../../tests/rtlcheck/SC/" -maxdepth 1 -name \*.test); do
+    file_chop=$(basename $file)
+    file_chop="${file_chop%.*}"
+    echo "Running test $file_chop"
+    ../../src/rtlcheck -v 7 -i $file -o pc_out/$file_chop.out \
+    -m ../../uarches/Vscale.uarch -t sva/${file_chop}_rtl.out
+    sed -e "s/TEST_NAME/${file_chop}/g" job_template.sh > jobs/job_${file_chop}.sh
+    sed -e "s/SIM_TOP_NAME/vscale_sim_top_${file_chop}.v/g" FPV_template_full_proof.tcl > fpv/FPV_cmdline_${file_chop}.tcl
+done
+
+rm -rf rtlcheck_tarball.tgz
+tar czvf rtlcheck_tarball.tgz fpv/ jg_out/ jobs/ pc_out/ sva/
