scripts/rtlcheck/job_template.sh
@@ -1,0 +1,28 @@
+#!/bin/bash
+# parallel job using 5 cores. and runs for 12 hours (max)
+#SBATCH -N 1   # node count
+#SBATCH --ntasks-per-node=4
+#SBATCH -t 12:00:00
+#SBATCH --mem=120G
+# sends mail when process begins, and 
+# when it ends. Make sure you define your email 
+# address.
+#SBATCH --mail-type=begin
+#SBATCH --mail-type=end
+#SBATCH --mail-user=<Your email address>
+TARBALL_DIR=<Directory where the tarball of assertions and Tcl scripts is>
+VSCALE_DIR=<Vscale root directory>
+PROJ_ROOT_DIR=<JasperGold project root directory>
+
+cd ${VSCALE_DIR}/src/main/verilog/
+# Add the RTL for the test
+{ head -n -1 vscale_sim_top_unmod.v; cat ${TARBALL_DIR}/sva/TEST_NAME_rtl.out; tail -n 1 vscale_sim_top_unmod.v; } > vscale_sim_top_TEST_NAME.v
+
+# Return to Vscale root directory.
+cd ../../..
+
+# Run JasperGold.
+jg -no_gui -fpv ${TARBALL_DIR}/fpv/FPV_cmdline_TEST_NAME.tcl -proj ${PROJ_ROOT_DIR}/proj_dir_TEST_NAME/|tee ${TARBALL_DIR}/jg_out/TEST_NAME.txt
+
+# Remove the project directory.
+rm -rf ${PROJ_DIR}/proj_dir_TEST_NAME/
